\documentclass{article}
\topmargin = -0.5in
\oddsidemargin = 0in
\evensidemargin = \oddsidemargin
\textwidth = 6.5in
\textheight = 9in
\usepackage{times}
\usepackage{bcprules}
\usepackage{amsthm}
\usepackage{amsmath}
\newcommand{\mathType}[2]{\mathtt{#1}:\mathtt{#2}}

\newcommand{\step}[2]{{\tt #1} $\longrightarrow$ {\tt #2}}

\newcommand{\inferrule}[3]{\infrule[#1]{\mbox{#2}}{\mbox{#3}}}
\newcommand{\inferax}[2]{\infrule[#1]{\mbox{}}{\mbox{#2}}}

\newtheorem{example}{Example}

\title{Homework 3}

\author{Yan-Ru Jhou, Nurrachman Liu}

\date{Feb 7th, 2020}

\begin{document}

    \maketitle

    \begin{description}
        \item[4]{Sol}\\
            \begin{enumerate}
                \item[(a)] { \tt f (if x then 0 else 1)}\\
                    \begin{equation*}
                        \Gamma = \{ \mathType{x}{Bool}, \mathType{f}{Int \rightarrow T} \}
                    \end{equation*}
                            \inferrule{T-APP}{
                                $\cfrac{\Gamma(f) = T}{\Gamma \vdash \text{f} :  \text{Int} \rightarrow \text{T}}$(T-Var)
                                 \andalso
                                $\cfrac{ \cfrac{\Gamma(x) = Bool}{\Gamma \vdash \text{x} : \text{Bool}}\text{(T-Var)} \quad \cfrac{}{0:\text{Int}}\text{(T-Num)} \quad  \cfrac{}{1:\text{Int}}\text{(T-Num)} }{\Gamma \vdash \text{if x then 0 else 1} :  \text{Int}}$(T-IF)
                            }{$\Gamma \vdash \text{f (if x then 0 else 1)} : \text{T} $}
                \item[(b)] {\tt f (if (f x) then 0 else 1)}
                    \begin{equation*}
                                   \Gamma = \{ \mathType{x}{Int}, \mathType{f}{Int \rightarrow Bool} \}
                    \end{equation*}
                \inferrule{T-APP}{
                    $\cfrac{\Gamma(f):Int\rightarrow T}{\Gamma \vdash \text{f} :  \text{Int} \rightarrow \text{T}}$(T-Var)
                    \andalso
                    $\cfrac{ \cfrac{ \cfrac{\Gamma(f):Int\rightarrow T}{\Gamma \vdash \text{f} : \text{Int} \rightarrow \text{Bool} }\text{(T-Var)} \quad \cfrac{\Gamma(x):Int}{\Gamma \vdash \text{x : Int}}\text{(T-Var)}  }{\Gamma \vdash \text{f x} : \text{Bool}}\text{(T-App)} \quad \cfrac{}{0:\text{Int}}\text{(T-Num)} \quad  \cfrac{}{1:\text{Int}}\text{(T-Num)} }
                    {\Gamma \vdash \text{f (if (f x) then 0 else 1)} :  \text{Int}}$(T-IF)
                    }{$\Gamma \vdash \text{f (if (f x) then 0 else 1)} : \text{T} $}
                \item[(c)] {\tt f (if (f x) then (f 0) else 1)}\\
                    No. the type of f  has to be $Int \rightarrow Int$ in $t2$ and $T \rightarrow Bool$ in $t1$ at the same time
            \end{enumerate}

        \item [5]{Sol}
            \begin{enumerate}
                \item[(a)]{Proof of Progressive Theorem} \\
                    By induction on the derivation of t:T\\
                    \textit{Induction hypothesis:} If $\Gamma \vdash t_0:T_0$, where $\Gamma \vdash t_0:T_0$ is a sub-derivation of $\Gamma \vdash t:T$, then either $t_0$ is a value or exists $t_0'$ such that  $t_0$ $\rightarrow$ $t_0'$
                    \begin{proof}
                        Case analysis on the root rule in $\Gamma \vdash t:T$.
                        \begin{itemize}
                            \item Case T-VAR: Then t = x, which is a value
                            \item Case T-FUN: Then t = function x:T $\rightarrow$ t , which is a value
                            \item Case T-APP: Then t = $t_1$ $t_2$, where $\Gamma \vdash t_1 t_2 :T$, $\Gamma \vdash t_1:T2 \rightarrow T $, and $\Gamma \vdash t_2:T2$. \\
                                By IH, $t_1$ is either a value or there exists $t_1'$ such that $t_1$ $\rightarrow$ $t_1'$, and $t_2$ is either a value or there exists $t_2'$ such that $t_2$ $\rightarrow$ $t_2'$\\
                                IF $t_1$ is a value, by CFL, $t_1$ has the value v1 with the form $function\ x:T_{12} \rightarrow t_{12}$\\
                                IF $t_2$ is a value, by CFL, $t_2$ has the value v1 with the form $function\ x:T_{22} \rightarrow t_{22}$\\
                                Case analysis on $t_1$ and $t_2$
                                \begin{itemize}
                                    \item Case exists $t_1'$ such that $t_1$ $\rightarrow$ $t_1'$:\\
                                        Then $t_1\ t_2$ $\rightarrow$ $t_1'\ t_2$ by E-APP1
                                    \item Case $t_1$ is a value $v_1$ and exists $t_2'$ such that $t_2$ $\rightarrow$ $t_2'$\\
                                        Then $t \rightarrow t' = v_1 t_2'$ by E-APP2
                                    \item Case Both $t_1$ and $t_2$ are values\\
                                        Then, $t \rightarrow t' = [x \rightarrow v_2]t_{12}$ by E-APPBETA
                                \end{itemize}
                        \end{itemize}
                    \end{proof}
                \item[(b)]{Arbitrary Type Environment}\\ let $t_1 = true$ , $t_2 = \text{function \ } y:Bool \rightarrow y $, and $\Gamma = \{(t_1,Bool \rightarrow true)\}$\\
                   Then $\Gamma \vdash t_1 t_2: bool$ , but $t_1 t_2$ cannot step
                \item[(c)]{Proof of Preservation Theorem}\\
                    By induction on the derivation of $\Gamma \vdash t:T$\\
                    \textit{Induction hypothesis:} If $\Gamma \vdash t_0:T_0$ and $t_0$ $\rightarrow$ $t_0'$, where $\Gamma \vdash t_0:T_0$ is a sub-derivation of $\Gamma \vdash t:T$, then $\Gamma \vdash t_0':T_0$
                    \begin{proof}
                        Case analysis on the root rule in $\Gamma \vdash t:T$.
                        \begin{itemize}
                            \item Case T-VAR: Then $t = x$,and $x:T \in \Gamma$.Contradiction ($t$ cannot step)
                            \item Case T-ABS: Then $t = \text{function\ } x:T_1 \rightarrow t_2 $.Contradiction($t$ cannot step)
                            \item Case T-APP: Then $t = t_1 t_2$, $\Gamma \vdash t_1: T_{11} \rightarrow T_{12}$,\space  $\Gamma \vdash t_2:T_{11}$,\space and $T=T_{12}$\\
                            Subcase analysis on $t \rightarrow t'$
                            \begin{itemize}
                                \item Case E-APP1: Then $t_1 \rightarrow t_1'$ , $t' = t_1't_2$\\
                                    Since $\Gamma \vdash t_1:T_{11} \rightarrow T_{12}$,and $t_1 \rightarrow t_1'$,\\
                                    By IH, $\Gamma \vdash t1':T_{11}\rightarrow T_{12}$.
                                    So, $\Gamma \vdash t':T_{12} = T$ by T-APP
                                \item Case E-APP2: Then $t_1 = v_1$, $t_2 \rightarrow t2'$, $t'=v_1 v_2'$\\ Similar
                                \item Case E-APPBETA: Then $t_1 = \text{function\ } x:T_{11} \rightarrow t_{12}$, $t_2 = v_{12}$, $t' = [x \rightarrow v_{12}]t_{12}$\\
                                    By Inversion Lemma, $\Gamma, x:T_{12} \vdash t_{12}:T_{12}$.\\So, by type substitution lemma, $\Gamma \vdash [x \rightarrow v_{12}]:T_{12} = T$
                            \end{itemize}
                        \end{itemize}
                    \end{proof}
            \end{enumerate}
        \item[6]{Sol}
            \begin{enumerate}
                \item [(a)]{Small-Step Operational Semantics }
                    \inferrule{E-FOR1}{\step{t$_1$}{t$_1'$}}
                    {\step{for t$_1$ do t$_2$}{for t$_1'$ do t$_2$}}
                    \inferrule{E-FORRED1}{ cond = n $[\![>]\!]$ 0 \andalso n' = n $[\![-]\!]$ 1 }
                    {\step{for n do t$_2$}{ if cond then for n' do t$_2$ else ()}}
                \item[(b)]{Typing Rule }
                    \inferrule{T-FOR}{$\Gamma \vdash t_1:\text{int}$ \andalso $\Gamma \vdash t_2:\text{T}$}
                    { $\Gamma \vdash$ for t$_1$ do t$_2$:Unit}
            \end{enumerate}

    \end{description}

%    \section{Language of Booleans and Integers}
%
%    \subsection{Syntax}
%
%    \begin{tt}
%        \begin{tabular}{rrl}
%            t & ::= & b $\mid$ if t then t else t \\
%            &$\mid$& n $\mid$ t + t $\mid$ t > t \\
%            b & ::= & true $\mid$ false \\
%            n & ::= & \mbox{\rm integer constant} \\
%            v & ::= & b $\mid$ n \\
%        \end{tabular}
%    \end{tt}
%
%
%    \subsection{Small-Step Operational Semantics}
%
%
%    \inferax{E-IfTrue}{\step{if true then t$_2$ else t$_3$}{t$_2$}}
%
%    \inferax{E-IfFalse}{\step{if false then t$_2$ else t$_3$}{t$_3$}}
%
%    \inferrule{E-If}{\step{t$_1$}{t$_1'$}}
%    {\step{if t$_1$ then t$_2$ else t$_3$}{if t$_1'$ then t$_2$ else t$_3$}}
%
%
%    \inferrule{E-Plus1}{\step{t$_1$}{t$_1'$}}
%    {\step{t$_1$ + t$_2$}{t$_1'$ + t$_2$}}
%
%
%    \inferrule{E-Plus2}{\step{t$_2$}{t$_2'$}}
%    {\step{v$_1$ + t$_2$}{v$_1$ + t$_2'$}}
%
%
%    \inferrule{E-PlusRed}{n = n$_1$ $[\![+]\!]$ n$_2$}
    %%    {\step{n$_1$ + n$_2$}{n}}
%
%    \inferrule{E-GT1}{\step{t$_1$}{t$_1'$}}
%    {\step{t$_1$ > t$_2$}{t$_1'$ > t$_2$}}
%
%
%    \inferrule{E-GT2}{\step{t$_2$}{t$_2'$}}
%    {\step{v$_1$ > t$_2$}{v$_1$ > t$_2'$}}
%
%
%    \inferrule{E-GTRed}{b = n$_1$ $[\![>]\!]$ n$_2$}
%    {\step{n$_1$ > n$_2$}{b}}


\end{document}
